add route callback family bridges

rocq/theories/TypeSystem/TypeSafetyDirectCallRoute.v
@@ -640,6 +640,70 @@ Definition eval_preserves_typing_roots_store_safe_synthetic_direct_call_ready_bo
     store_no_shadow s_body /\
     root_env_no_shadow R_body.
 
+
+Definition eval_preserves_typing_roots_store_safe_synthetic_direct_call_ready_body_call_callback_height_statement_in_env_family
+    (env_family : global_env -> Prop) : Prop :=
+  forall env,
+    env_family env ->
+  forall fname fdef fcall used used' s_args s_body vs ret R_args
+      arg_roots fname_body args_body T_body Gamma_out R_body roots_body,
+    In fdef (env_fns env) ->
+    fn_name fdef = fname ->
+    alpha_rename_fn_def used fdef = (fcall, used') ->
+    direct_call_target_expr (fn_body fcall) =
+      Some (fname_body, args_body, ECall fname_body args_body) ->
+    preservation_ready_args args_body ->
+    typed_env_roots (global_env_with_local_bounds env (fn_bounds fcall))
+      (fn_outlives fcall) (fn_lifetimes fcall)
+      (call_param_root_env (fn_params fcall) arg_roots R_args)
+      (sctx_of_ctx (params_ctx (fn_params fcall)))
+      (ECall fname_body args_body) T_body (sctx_of_ctx Gamma_out) R_body
+      roots_body ->
+    fn_env_unique_by_name (global_env_with_local_bounds env (fn_bounds fcall)) ->
+    fn_root_shadow_synthetic_direct_call_ready_summary_evidence_at
+      (global_env_with_local_bounds env (fn_bounds fcall)) fname_body ->
+    direct_call_callee_body_root_synthetic_direct_call_ready_evidence_at
+      (global_env_with_local_bounds env (fn_bounds fcall)) fname_body ->
+    store_typed_prefix (global_env_with_local_bounds env (fn_bounds fcall))
+      (bind_params (fn_params fcall) vs s_args)
+      (sctx_of_ctx (params_ctx (fn_params fcall))) ->
+    store_roots_within
+      (call_param_root_env (fn_params fcall) arg_roots R_args)
+      (bind_params (fn_params fcall) vs s_args) ->
+    store_no_shadow (bind_params (fn_params fcall) vs s_args) ->
+    root_env_no_shadow
+      (call_param_root_env (fn_params fcall) arg_roots R_args) ->
+    root_env_store_roots_named
+      (call_param_root_env (fn_params fcall) arg_roots R_args)
+      (bind_params (fn_params fcall) vs s_args) ->
+    root_env_store_keys_named
+      (call_param_root_env (fn_params fcall) arg_roots R_args)
+      (bind_params (fn_params fcall) vs s_args) ->
+    eval (global_env_with_local_bounds env (fn_bounds fcall))
+      (bind_params (fn_params fcall) vs s_args)
+      (ECall fname_body args_body) s_body ret ->
+    forall n_body_call,
+    direct_call_eval_height
+      (global_env_with_local_bounds env (fn_bounds fcall))
+      (bind_params (fn_params fcall) vs s_args)
+      (ECall fname_body args_body) s_body ret n_body_call ->
+    store_typed_prefix (global_env_with_local_bounds env (fn_bounds fcall))
+      s_body (sctx_of_ctx Gamma_out) /\
+    value_has_type (global_env_with_local_bounds env (fn_bounds fcall))
+      s_body ret T_body /\
+    store_ref_targets_preserved
+      (global_env_with_local_bounds env (fn_bounds fcall))
+      (bind_params (fn_params fcall) vs s_args) s_body /\
+    store_roots_within R_body s_body /\
+    value_roots_within roots_body ret /\
+    store_no_shadow s_body /\
+    root_env_no_shadow R_body.
+
+Definition eval_preserves_typing_roots_store_safe_synthetic_direct_call_ready_body_call_callback_height_statement_in_local_bounds_family
+    (base : global_env) : Prop :=
+  eval_preserves_typing_roots_store_safe_synthetic_direct_call_ready_body_call_callback_height_statement_in_env_family
+    (global_env_local_bounds_family base).
+
 Definition eval_preserves_typing_roots_store_safe_synthetic_direct_call_ready_summary_at_prefix_call_statement_evidence_at_height_statement
     : Prop :=
   forall env s fname args s' v n_call,
@@ -10284,6 +10348,102 @@ Proof.
       Hrn_bind Hnamed_bind Hkeys_bind Heval_nested n_body_call
       Hheight_nested _Hlt.
     eapply Hbody_call_callback_height; eassumption.
+Qed.
+
+
+Theorem eval_preserves_typing_roots_store_safe_synthetic_direct_call_ready_summary_at_prefix_call_statement_evidence_at_height_statement_in_env_family_of_body_call_callback_height :
+  eval_preserves_frame_param_scope_synthetic_direct_call_ready_statement ->
+  eval_preserves_typing_ready_prefix_mutual_statement ->
+  eval_preserves_typing_roots_ready_prefix_mutual_statement ->
+  eval_preserves_roots_ready_mutual_statement ->
+  eval_preserves_root_names_ready_mutual_statement ->
+  eval_preserves_root_keys_named_ready_mutual_statement ->
+  forall env_family,
+  (forall env fname fdef fcall used used' fname_body args_body synthetic_body,
+    env_family env ->
+    In fdef (env_fns env) ->
+    fn_name fdef = fname ->
+    alpha_rename_fn_def used fdef = (fcall, used') ->
+    direct_call_target_expr (fn_body fcall) =
+      Some (fname_body, args_body, synthetic_body) ->
+    fn_root_shadow_synthetic_direct_call_ready_summary_evidence_at
+      (global_env_with_local_bounds env (fn_bounds fcall)) fname_body) ->
+  (forall env fname fdef fcall used used' fname_body args_body,
+    env_family env ->
+    In fdef (env_fns env) ->
+    fn_name fdef = fname ->
+    alpha_rename_fn_def used fdef = (fcall, used') ->
+    direct_call_target_expr (fn_body fcall) =
+      Some (fname_body, args_body, ECall fname_body args_body) ->
+    fn_body fcall = ECall fname_body args_body) ->
+  eval_preserves_typing_roots_store_safe_synthetic_direct_call_ready_body_call_callback_height_statement_in_env_family
+    env_family ->
+  eval_preserves_typing_roots_store_safe_synthetic_direct_call_ready_summary_at_prefix_call_statement_evidence_at_height_statement_in_env_family
+    env_family.
+Proof.
+  intros Hscope_synthetic Htyping_prefix Hprefix_ready Hroots_ready
+    Hroot_names Hroot_keys env_family Hsummary_body_at_all Hbody_exact
+    Hbody_call_callback_height.
+  unfold
+    eval_preserves_typing_roots_store_safe_synthetic_direct_call_ready_summary_at_prefix_call_statement_evidence_at_height_statement_in_env_family,
+    eval_preserves_typing_roots_store_safe_synthetic_direct_call_ready_summary_at_prefix_call_statement_evidence_at_height_statement_in_env.
+  intros env Henv s fname args s' v n_call Heval_call Hheight_call Omega n
+    R Sigma T Sigma' R' roots Hsafe_args Hstore Hroots Hshadow Hrn Hnamed
+    Hkeys Htyped Hunique Hsummary_at Hevidence_at.
+  eapply
+    eval_preserves_typing_roots_store_safe_synthetic_direct_call_ready_ecall_cleanup_bridge_with_alpha_evidence_at_decreasing_body_call_callback_prefix_store_final_roots_core_exact_body;
+    try eassumption.
+  - intros fdef fcall used used' fname_body args_body synthetic_body
+      Hin Hname Hrename Htarget.
+    eapply Hsummary_body_at_all; eassumption.
+  - intros fdef fcall used used' fname_body args_body
+      Hin Hname Hrename Htarget.
+    eapply Hbody_exact; eassumption.
+  - intros fdef fcall used used' s_args s_body vs ret R_args arg_roots
+      fname_body args_body T_body Gamma_out R_body roots_body Hin Hname
+      Hrename Htarget_body Hready_body Htyped_body Hunique_body
+      Hsummary_body Hevidence_body Hstore_bind Hroots_bind Hshadow_bind
+      Hrn_bind Hnamed_bind Hkeys_bind Heval_nested n_body_call
+      Hheight_nested _Hlt.
+    eapply Hbody_call_callback_height; eassumption.
+Qed.
+
+Theorem eval_preserves_typing_roots_store_safe_synthetic_direct_call_ready_summary_at_prefix_call_statement_evidence_at_height_statement_in_local_bounds_family_of_body_call_callback_height :
+  eval_preserves_frame_param_scope_synthetic_direct_call_ready_statement ->
+  eval_preserves_typing_ready_prefix_mutual_statement ->
+  eval_preserves_typing_roots_ready_prefix_mutual_statement ->
+  eval_preserves_roots_ready_mutual_statement ->
+  eval_preserves_root_names_ready_mutual_statement ->
+  eval_preserves_root_keys_named_ready_mutual_statement ->
+  forall base,
+  (forall env fname fdef fcall used used' fname_body args_body synthetic_body,
+    global_env_local_bounds_family base env ->
+    In fdef (env_fns env) ->
+    fn_name fdef = fname ->
+    alpha_rename_fn_def used fdef = (fcall, used') ->
+    direct_call_target_expr (fn_body fcall) =
+      Some (fname_body, args_body, synthetic_body) ->
+    fn_root_shadow_synthetic_direct_call_ready_summary_evidence_at
+      (global_env_with_local_bounds env (fn_bounds fcall)) fname_body) ->
+  (forall env fname fdef fcall used used' fname_body args_body,
+    global_env_local_bounds_family base env ->
+    In fdef (env_fns env) ->
+    fn_name fdef = fname ->
+    alpha_rename_fn_def used fdef = (fcall, used') ->
+    direct_call_target_expr (fn_body fcall) =
+      Some (fname_body, args_body, ECall fname_body args_body) ->
+    fn_body fcall = ECall fname_body args_body) ->
+  eval_preserves_typing_roots_store_safe_synthetic_direct_call_ready_body_call_callback_height_statement_in_local_bounds_family
+    base ->
+  eval_preserves_typing_roots_store_safe_synthetic_direct_call_ready_summary_at_prefix_call_statement_evidence_at_height_statement_in_local_bounds_family
+    base.
+Proof.
+  intros Hscope_synthetic Htyping_prefix Hprefix_ready Hroots_ready
+    Hroot_names Hroot_keys base Hsummary_body_at_all Hbody_exact
+    Hbody_call_callback_height.
+  eapply
+    eval_preserves_typing_roots_store_safe_synthetic_direct_call_ready_summary_at_prefix_call_statement_evidence_at_height_statement_in_env_family_of_body_call_callback_height;
+    eassumption.
 Qed.
 
 Theorem eval_preserves_typing_roots_synthetic_direct_call_ready_summary_at_prefix_call_statement_evidence_at_height_statement_of_exact_body_call_route_package :
